Enhancements to imperative.dfy.

dafny/imperative.dfy
@@ -43,35 +43,180 @@ module imperative
     }
 
     /*
-    Can the incorporation of machine-checkable
-    logical specifications in code help us to
-    avoid such errors? The answer is yes. Let's
-    see how.
-
-    /*
     Here's an imperative program for computing factorial.
     */
     method verified_factorial(n: nat) returns (f: nat) 
         ensures f == fact(n)
     {
+        // If base case, return result without recursion
         if (n == 0) 
         { 
             return 1;
         }
-        var t: nat := n;
-        var a: nat := 1;
-        while (t !=  0)
-            invariant 0 <= t <= n
-            invariant fact(n) == a * fact(t) 
-        {
-            a := a * t;
-            t := t - 1;
-        }
-        // here we know fact(n) == a * fact(t) AND t == 0
-        // from these two facts we can conclude that a == what?
-        return a;
-    }
 
+        // The rest of the code handles recursive case
+        assert n > 0;
+
+        /*
+           Strategy: use a while loop to compute the
+           answer. We can do this by using a variable,
+           a, to hold a "partial factorial value" in
+           the form of a product of the numbers from 
+           n down to a loop index, "i," that we start
+           at n and decrement down, terminating the
+           loop when n==0. At each point just before,
+           during, and right after the loop, a is a
+           product of the numbers from n down to i, 
+           and the value of i represents how much of
+           this product-computing work remains to be
+           done. So, for example, if we're computing
+           factorial(10) and a holds the value 10 * 9,
+           then i must be 8 because multiplying a by
+           the factors from 8 down to 1 remains to be
+           done. A critical "invariant" then is that
+           if you multiply a by the factorial of i 
+           you get the final answer, which is to say
+           the factorial of n.  
+        */
+
+        /* 
+           Step 1. Set up state for the loop to work.
+
+           We first initializie a := 1 and i := n and
+           check that the invariant holds. Note that
+           we are using our pure functional math-like
+           definition of fact as a *specification* of
+           the factorial function we're implementing.
+        */
+        var i: nat := n;    // nat type of i explicit
+        var a := 1;         // can let Dafny infer it
+
+        /*
+           In Dafny, we can use matnematical logic to
+           express what must be true at any given point
+           in the execution of a program in the form of
+           an "assertion." Here we assert that our loop
+           invariant holds. The Dafny verifier tries to
+           prove that the assertion is a true propsition
+           about the state of the program when control
+           reaches this point in the execution of this
+           program.
+        */
+        assert a * fact(i) == fact(n); // "invariant"
+
+
+        /*
+            Step 2: Now evaluate the loop to get the
+            answer.
+
+           To evaluate a loop, first, evaluate the 
+           loop condition (i > 0).Then , if the result 
+           is false, terminate the loop. Otherwise, 
+           evaluate the loop body, then iterate (run 
+           the loop again, starting by evaluating the
+           loop condition).     
+        */
+
+        /*
+           Note that we can deduce that the loop body
+           is going to execute at least once. It will 
+           run if i > 0. What is i? We initialized it
+           to n and haven't change it since then so it
+           must still be equal to n. Do we know that 
+           n is greater than 0? We do, because (1) it
+           can't be negative owning to its type, and 
+           (2) it can't be 0 because if it were 0 the
+           program would already have returned. But we
+           can now do better than just reasoning in our
+           heads; we can use logic to express what we
+           believe to be true and let Dafny try to 
+           check it for us automatically.
+        */
+        assert i > 0;
+        
+        /*
+        Let's just think briefly about cases. We know
+        i can't be zero. It could be one. If it's one,
+        then the loop body will run. The loop body will
+        run. a, which starts at 1, will be multiplied 
+        by i, which is 1, then i will be decremented.
+        It will have the value 0 and the loop will not
+        run again, leaving a with the value 1, which 
+        is the right answer. So, okay, let's run the
+        loop.
+        */
+        
+        while (i >  0)
+            invariant 0 <= i <= n
+            invariant fact(n) == a * fact(i) 
+        {
+            a := a * i;
+            i := i - 1;
+        }
+
+        /*
+           At this point, we know that the loop 
+           condition is false. In English, we'd
+           say it is no longer true that i is greater
+           than zero." We can do better that saying
+           this in natural language then forgetting
+           it. We can use formal logic to formalize 
+           and document our belief and if we do this
+           then Dafny pays us well for our effort 
+           by checking that our assertion is true. 
+        */
+        assert !(i > 0);
+
+        /*
+            We can also have Dafny check that our
+            loop invariant still holds. 
+        */
+        assert a * fact(i) == fact(n);
+
+        /*
+            And now comes the most crucial step of 
+            all in our reasoning. We can deduce that
+            a now holds the correct answer. That this
+            is so follows from the conjunction of the
+            two assertions we just made. First, that
+            i is not greater than 0 and given that its
+            type is nat, the only possible value it
+            can have now is 0. And that's what we'd
+            expect, because that's the condition on
+            which the loop terminates, which is just
+            did! But better than just saying it, let
+            us also formalize, document, and check it.
+        */
+        assert i == 0;
+
+        /*
+           Now it's easy to see. No matter what value
+           i has, a * fact(i) == fact(n), and i == 0, so
+           we have a * fact(0) == fact(n), and we know
+           that fact(0) is 1 because we see that in the
+           very mathematical definition of fact, so it
+           must be that a = fact(n). Dafny can check!
+         */
+        assert a == fact(n);
+
+        /*
+            We thus have the answer we need to return.
+            Dafny verifies that our program satisfies
+            its formal specification. We no longer have
+            to pray. We *know* that our program is right
+            and Dafny confirms our belief.
+        */
+        return a;
+
+        /*
+            Mathematical logic is to software as the 
+            calculus is to physics and engineering.
+            It's not just an academic curiosity. It is
+            a critical intellectual tool, inceasingly
+            being used for precise for specification 
+            and verification of practical programs.
+        */
+    }
 
     /*
     Similarly, here an imperative implementation 
@@ -79,28 +224,110 @@ module imperative
     */
     method fibonacci(n: nat) returns (r: nat)
     {
-        if (n < 2) return n;
-        var fib_minus_2 := 0;
-        var fib_minus_1 := 1;
-        var fib_current := 0;
-        var ind := 2;
-        while (ind <= n) 
+        /*
+            Represent values for two base cases.
+        */
+        var fib0, fib1 := 0, 1; //parallel assmt
+
+        /*
+           Return base case result if appropriate
+        */
+        if (n == 0) { return fib0; }
+        if (n == 1) { return fib1; }
+
+        /*
+           At this point, we know n (a nat) >= 2.
+        */
+        assert n >= 2;
+
+        /*
+           Our strategy for computing fib(n) is
+           to use a while loop with an index i.
+           Our design will be based on the idea
+           that at the beginning and end of each 
+           loop iteration, that we have computed
+           fib(i) and that its value is stored in
+           fib1. Then within the loop body we'll 
+           compute fib(i+1) and then increment i.
+ 
+           At this point, we've already computed
+           fib(0), stored in fib0, and and fib(1), 
+           in fib1, so we should initialize i to 
+           be 1. 
+           
+           We'll want to terminate the loop when 
+           i == n, at which point fib1 should
+           have the value fib(i), where i ==n,
+           so fib(i) will be fib(n). That is the
+           strategy. So let's go.
+        */
+        var i := 1;
+
+        /*
+            We can state and Dafny can verify a
+            number of conditions that we expect
+            and require to hold at this point.
+        */
+        assert fib1 == fib(i);
+        assert fib0 == fib(i-1);
+        assert i <= n;
+
+
+        /*
+            Here's the loop. We can be sure it will
+            run at least once, because at this point
+            n must be greater than or equal to 2 ...
+        */
+        assert n >= 2;
+        /*
+            and we know that i is 1, and 1 < 2, which
+            satisfies the loop condition. If n were to
+            be equal to 2, the loop body would run, the
+            value of fib2 would be set to the sum of 
+            the current values of fib1 and fib0, giving
+            us fib2; then fib0 will be set to the current
+            value of fib1, fib1 will be set of the value
+            of fib2, and i will be incremented, at which
+            point the critical condition will be restored: 
+            fib1 == fib(i), but where i is now equal to 2.
+            We also know that i started off less than n,
+            it gets incremented by only 1 each time the
+            loop body executes, and the loop terminates
+            when it is no longer true that i < n. So it
+            remains true at all times that i <= n. For
+            Dafny to be able to verify that a loop does
+            what it's meant to do, we have to declare 
+            the invariants that are required to hold.
+        */
+        while (i < n) 
+            invariant i <= n;
+            invariant fib0 == fib(i-1);
+            invariant fib1 == fib(i);
         {
-            fib_current := fib_minus_2 + fib_minus_1;
-            fib_minus_2 := fib_minus_1;
-            fib_minus_1 := fib_current;
-            ind := ind + 1;
+            var fib2 := fib0 + fib1;
+            fib0 := fib1;
+            fib1 := fib2;
+            i := i + 1;
         }
-        return fib_current;
+        /*
+            So we know that every iteration of the loop
+            body has preserved the condition that fib1 is
+            equal to fib(i). What else do we know? Well,
+            a little bit of logical reasoning leads us to
+            conclude that i == n. Combining these facts
+            then leads to the final result: fib1==fib(n)
+        */
+        assert i <= n;      // invariant
+        assert !(i < n);    // loop condition is false
+        assert (i <= n) && !(i < n) ==> (i == n);
+        assert i == n;      // deductive conclusion
+        assert fib1 == fib(i); // invariant
+        assert fib1 == fib(i) && (i==n) ==> fib1 == fib(n);
+        assert fib1 == fib(n);
+
+        /*
+            We now have a proven-correct result!
+        */
+        return fib1;
     }
-
-
-    method verified-fibonacci(n: nat) returns (r: nat)
-        ensures r == fib(n)
-    /* a verified implementation goes here! */
-
 }
-
-
-
-
